theories/examples/template_adequacy_concurrency.v
@@ -1,0 +1,79 @@
+From iris.algebra Require Import auth agree excl gmap gset frac.
+From iris.proofmode Require Import tactics.
+From iris.base_logic Require Import invariants.
+From iris.program_logic Require Import adequacy.
+From cap_machine Require Import
+     stdpp_extra iris_extra
+     rules logrel fundamental.
+From cap_machine.examples Require Import addr_reg_sample.
+From cap_machine.examples Require Export mkregion_helpers disjoint_regions_tactics.
+
+Record prog := MkProg {
+  prog_start: Addr;
+  prog_end: Addr;
+  prog_instrs: list Word;
+
+  prog_size:
+    (prog_start + length prog_instrs)%a = Some prog_end;
+}.
+
+Definition prog_region (P: prog): gmap Addr Word :=
+  mkregion (prog_start P) (prog_end P) (prog_instrs P).
+
+Lemma prog_region_dom (P: prog):
+  dom (gset Addr) (prog_region P) =
+  list_to_set (finz.seq_between (prog_start P) (prog_end P)).
+Proof.
+  rewrite /prog_region /mkregion dom_list_to_map_L fst_zip //.
+  rewrite finz_seq_between_length /finz.dist.
+  pose proof (prog_size P). solve_addr.
+Qed.
+
+
+Lemma filter_dom_is_dom (m: gmap Addr Word) (d: gset Addr):
+  d ⊆ dom (gset Addr) m →
+  dom (gset Addr) (filter (λ '(a, _), a ∈ d) m) = d.
+Proof.
+  intros Hd. eapply set_eq. intros a.
+  rewrite (dom_filter_L _ _ d); auto.
+  intros. split; intros H.
+  { rewrite elem_of_subseteq in Hd |- * => Hd. specialize (Hd _ H).
+    eapply elem_of_gmap_dom in Hd as [? ?]. eexists. split; eauto. }
+  { destruct H as [? [? ?] ]; auto. }
+Qed.
+
+
+Program Definition all_cores :=
+  finz.seq
+    (@finz.FinZ machine_base.CoreNum 0 _ _)
+    (BinIntDef.Z.to_nat machine_base.CoreNum).
+Next Obligation.
+  pose machine_base.CorePos. lia.
+Qed.
+Next Obligation. lia. Qed.
+
+Definition init_cores : list cap_lang.expr :=
+  map (fun (i : CoreN) => (i, Seq (Instr Executable))) all_cores.
+
+Definition core_zero := (finz.FinZ 0
+                           all_cores_obligation_1
+                           all_cores_obligation_2).
+
+Definition is_initial_memory (mem_frags : list prog) (m: gmap Addr Word) :=
+  let region_list := map (fun f => prog_region f) mem_frags in
+  ⋃ region_list ⊆ m /\ disjoint_list_map region_list.
+
+Definition is_initial_registers
+  (P : prog) (reg: gmap (CoreN * RegName) Word) (i:CoreN) :=
+  reg !! (i, PC) = Some (WCap RWX (prog_start P) (prog_end P) (prog_start P))  (* PC *)
+  ∧ dom (gset (CoreN*RegName)) reg ⊆ (set_map (fun r => (i,r)) all_registers_s)
+  /\ (∀ (r: RegName), (i, r) ∉ ({[ (i, PC) ]} : gset (CoreN * RegName)) →
+                     ∃ (w:Word), reg !! (i, r) = Some w ∧ is_cap w = false).
+
+Definition is_initial_registers_with_adv
+  (P A : prog)
+  (r_adv : RegName)
+  (reg: gmap (CoreN * RegName) Word) (i:CoreN) :=
+  is_initial_registers P reg i
+  /\ reg !! (i, r_adv) = Some (WCap RWX (prog_start A) (prog_end A) (prog_start A)) (* adversary *)
+  /\ PC ≠ r_adv.
